\chapter{Logical Relations}

%%%%%%%%%%%%%%%%%%%%%%%%%%%%%%%%%%%%%%%%%%%%%%%%%%%%%%%%%%%%%%%%%%%%%%%%%%%%%%%
\section{Syntactic Provability and Semantic Truth}

% Some intuitions from propositional logic go here

\newcommand\Denot[1]{\llbracket#1\rrbracket}
\begin{alignat*}{2}
  \varphi & \Coloneqq \top \mid \bot \mid \varphi \to \varphi
\end{alignat*}

$\Denot{\cdot} \colon Formula \to D$
\begin{alignat*}{2}
  \Denot{\top} & = \texttt{true} \\
  \Denot{\bot} & = \texttt{false} \\
  \Denot{\varphi \to \psi} & = \Denot{\varphi} \Rightarrow \Denot{\psi}
\end{alignat*}

%%%%%%%%%%%%%%%%%%%%%%%%%%%%%%%%%%%%%%%%%%%%%%%%%%%%%%%%%%%%%%%%%%%%%%%%%%%%%%%
\section{Denotation of Types}

$\textbf{Type} = \mathcal{P}(Value_{\emptyset})$ (sets of closed values)

$\Denot{\cdot} \colon Type \to \textbf{Type}$ - denotation of a type - set of values of that type
\begin{alignat*}{2}
  \Denot{\texttt{Unit}} & = \{\texttt{()}\} \\
  \Denot{\tau_1 \to \tau_2} & = \{ v \mid \forall v' \in \Denot{\tau_1}\ldotp v\;v' \in \mathcal{E}\Denot{\tau_2} \}
\end{alignat*}

$\mathcal{E} \colon \textbf{Type} \to \mathcal{P}(Expr_{\emptyset})$

$\mathcal{E}R = \{ e \mid \forall e'\ldotp e \to^* e' \Rightarrow (\exists v \in R \ldotp e'=v) \lor (\exists e'' \ldotp e'\to^*e'') \}$

%%%%%%%%%%%%%%%%%%%%%%%%%%%%%%%%%%%%%%%%%%%%%%%%%%%%%%%%%%%%%%%%%%%%%%%%%%%%%%%
\section{The Logical Relation}

% From denotation of types to open expressions

$\Denot{\Gamma} = \{\gamma \mid \forall x\ldotp \gamma(x) \in \Denot{\Gamma(x)}\}$
($\gamma \in \Denot{\Gamma} \Longleftrightarrow \forall x\ldotp \gamma(x) \in \Denot{\Gamma(x)} $)

$\gamma \colon X \to Value_{\emptyset}$

$\Gamma \models e : \tau \Longleftrightarrow \forall \gamma \in \Denot{\Gamma}\ldotp \gamma^*(e) \in \mathcal{E}\Denot{\tau}$

%%%%%%%%%%%%%%%%%%%%%%%%%%%%%%%%%%%%%%%%%%%%%%%%%%%%%%%%%%%%%%%%%%%%%%%%%%%%%%%
\section{Soundness}

% Compatibility Lemmas, Fundamental Property, Adequacy, and Type Safety
% go here.
\newtheorem*{theorem}{Theorem}

\begin{theorem}[Fundamental Property]
  If $\Gamma \vdash e : \tau$ then $\Gamma \models e : \tau$
\end{theorem}

\begin{theorem}[Type safety]
  If $\emptyset \vdash e : \tau$ then $Safe(e)$

  $Safe(e) = \forall e'\ldotp e\to^*e' \Rightarrow (\exists v\ldotp e'=v) \lor (\exists e''\ldotp e'\to e'')$
\end{theorem}

\begin{theorem}[Adequacy]
  $\mathcal{E}R \subseteq Safe$
\end{theorem}

\newtheorem{lemma}{Lemma}

\begin{lemma}
  $\forall R \in \textbf{Type}\ldotp \forall v \in R\ldotp v \in \mathcal{E}R$
\end{lemma}

\begin{lemma}
  If $e \to e'$ and $e' \in \mathcal{E}R$ then $e \in \mathcal{E}R$
\end{lemma}

\begin{lemma}
  If $e_1 \in \mathcal{E}\Denot{\tau_2 \to \tau_1}$ and $e_2 \in \mathcal{E}\Denot{\tau_2}$ then $e_1\;e_2 \in \mathcal{E}\Denot{\tau_1}$

  Proof (sketch):

  Pick any $e'$ such that $e_1\;e_2 \to^* e'$

  i. $e_1 \to^* e_1'$ (not a value), then $e' = e_1'\;e_2$

  ii. $e_1 \to^* v_1$, $e_2\to e_2'$ (not a value) $e' = v_1\;e_2'$

  iii. $e_1 \to^* v_1$, $e_2 \to^* v_2$ and $v_1 v_2 \to^* e'$
\end{lemma}

\newtheorem{compatlemma}{Compatibility lemma}

\begin{compatlemma}
  $\Gamma \models () : Unit =$
\end{compatlemma}

\begin{compatlemma}
  $\Gamma \models x : \Gamma(x)$
\end{compatlemma}

\begin{compatlemma}
  If $\Gamma, x:\tau_1 \models e : \tau_2$ then $\Gamma \models \lambda x.e : \tau_1 \to \tau_2$
\end{compatlemma}

Proof sketch for Compatibility lemma 3:

Take any $\gamma \in \Denot{\Gamma}$

T.S. $\lambda^{\Uparrow*} e \in \mathcal{E}\Denot{\tau_1 \to \tau_2}$

From lemma 1:

T.S. $\lambda^{\Uparrow*} e \in \Denot{\tau_1 \to \tau_2}$

Take any $v \in \Denot{\tau_1}$

T.S. $(\lambda^{\Uparrow*} e)\;v \in \Denot{\tau_2}$

From lemma 2:

T.S. $(\gamma^{\Uparrow*} e)\{v/x\} \in \mathcal{E}\Denot{\tau_2}$

T.S. $(v \triangleleft \gamma)^* \in \mathcal{E}\Denot{\tau_2}$

From induction hypothesis:

T.S. $v \triangleleft \gamma \in \Denot{\Gamma, x : \tau_1}$

\begin{compatlemma}
  If $\Gamma \models e_1 : \tau_2 \to \tau_1 $ and $\Gamma \models e_2 : \tau_2$ then $\Gamma \models e_1\;e_2 : \tau_1$
\end{compatlemma}
Proof using lemma 3.

\medskip

Using Compatibility Lemmas proof of Fundamental Property is straightforward induction.

%%%%%%%%%%%%%%%%%%%%%%%%%%%%%%%%%%%%%%%%%%%%%%%%%%%%%%%%%%%%%%%%%%%%%%%%%%%%%%%
\section{Termination of Simply-Typed Lambda Calculus}

If $\emptyset \vdash e : \tau$ then $\exists v\ldotp e \to^* v$

To prove termination we will change definition of $\mathcal{E}$ to reflect that fact.

$\mathcal{E}R = \{ e \mid \exists v \in R\ldotp e \to^* v \}$

%%%%%%%%%%%%%%%%%%%%%%%%%%%%%%%%%%%%%%%%%%%%%%%%%%%%%%%%%%%%%%%%%%%%%%%%%%%%%%%
\section{Further Reading}
